\PassOptionsToPackage{unicode=true}{hyperref} % options for packages loaded elsewhere
\PassOptionsToPackage{hyphens}{url}
%
\documentclass[]{article}
\usepackage{lmodern}
\usepackage{amssymb,amsmath}
\usepackage{ifxetex,ifluatex}
\usepackage{fixltx2e} % provides \textsubscript
\ifnum 0\ifxetex 1\fi\ifluatex 1\fi=0 % if pdftex
  \usepackage[T1]{fontenc}
  \usepackage[utf8]{inputenc}
  \usepackage{textcomp} % provides euro and other symbols
\else % if luatex or xelatex
  \usepackage{unicode-math}
  \defaultfontfeatures{Ligatures=TeX,Scale=MatchLowercase}
\fi
% use upquote if available, for straight quotes in verbatim environments
\IfFileExists{upquote.sty}{\usepackage{upquote}}{}
% use microtype if available
\IfFileExists{microtype.sty}{%
\usepackage[]{microtype}
\UseMicrotypeSet[protrusion]{basicmath} % disable protrusion for tt fonts
}{}
\IfFileExists{parskip.sty}{%
\usepackage{parskip}
}{% else
\setlength{\parindent}{0pt}
\setlength{\parskip}{6pt plus 2pt minus 1pt}
}
\usepackage{hyperref}
\hypersetup{
            pdftitle={Untitled},
            pdfborder={0 0 0},
            breaklinks=true}
\urlstyle{same}  % don't use monospace font for urls
\usepackage[margin=1in]{geometry}
\usepackage{graphicx,grffile}
\makeatletter
\def\maxwidth{\ifdim\Gin@nat@width>\linewidth\linewidth\else\Gin@nat@width\fi}
\def\maxheight{\ifdim\Gin@nat@height>\textheight\textheight\else\Gin@nat@height\fi}
\makeatother
% Scale images if necessary, so that they will not overflow the page
% margins by default, and it is still possible to overwrite the defaults
% using explicit options in \includegraphics[width, height, ...]{}
\setkeys{Gin}{width=\maxwidth,height=\maxheight,keepaspectratio}
\setlength{\emergencystretch}{3em}  % prevent overfull lines
\providecommand{\tightlist}{%
  \setlength{\itemsep}{0pt}\setlength{\parskip}{0pt}}
\setcounter{secnumdepth}{0}
% Redefines (sub)paragraphs to behave more like sections
\ifx\paragraph\undefined\else
\let\oldparagraph\paragraph
\renewcommand{\paragraph}[1]{\oldparagraph{#1}\mbox{}}
\fi
\ifx\subparagraph\undefined\else
\let\oldsubparagraph\subparagraph
\renewcommand{\subparagraph}[1]{\oldsubparagraph{#1}\mbox{}}
\fi

% set default figure placement to htbp
\makeatletter
\def\fps@figure{htbp}
\makeatother


\title{Untitled}
\author{}
\date{\vspace{-2.5em}}

\begin{document}
\maketitle

\hypertarget{including-plots}{%
\subsection{Including Plots}\label{including-plots}}

\usepackage{mathrsfs}

\$\$\begin{align}
PL(\beta)&=\prod_{i=1}^{l}\frac{exp(\beta S_i)}{\sum_{l\in R_{D_i}(\tau_i)}exp(\beta S_l)}\\
logPL(\beta)&=\sum_{i=1}^{l}log\frac{exp(\beta S_i)}{\sum_{l\in R_{D_i}(\tau_i)}exp(\beta S_l)}\\
&=\sum_{i=1}^{l}\beta S_i-\sum_{i=1}^llog{\sum_{l\in R_{D_i}(\tau_i)}exp(\beta S_l)}\\

u(\beta)&=\frac{\partial logPL(\beta)}{\partial \beta}\\
&=\sum_{i=1}^{l}S_i-\sum_{i=1}^l\frac{\sum_{l\in R_{D_i}(\tau_i)}S_lexp(\beta S_l)}{\sum_{l\in R_{D_i}(\tau_i)}exp(\beta S_l)}\\
u(0)&=\sum_{i=1}^{l}S_i-\sum_{i=1}^l\frac{\sum_{l\in R_{D_i}(\tau_i)}S_l}{\sum_{l\in R_{D_i}(\tau_i)}1}\\

i(\beta)&=-\frac{\partial^2logPL(\beta)}{\partial \beta^2}\\
&=\sum_{i=1}^l\frac{(\sum_{l\in R_{D_i}(\tau_i)}S_l^2exp(\beta S_l))(\sum_{l\in R_{D_i}(\tau_i)}exp(\beta S_l))-(\sum_{l\in R_{D_i}(\tau_i)}S_lexp(\beta S_l))^2}{\{\sum_{l\in R_{D_i}(\tau_i)}exp(\beta S_l)\}^2}\\
i(0)&=\sum_{i=1}^l\frac{(\sum_{l\in R_{D_i}(\tau_i)}S_l^2)(\sum_{l\in R_{D_i}(\tau_i)}1)-(\sum_{l\in R_{D_i}(\tau_i)}S_l)^2}{\{\sum_{l\in R_{D_i}(\tau_i)}1\}^2}\\
\end{align}\textbackslash{}

\[
Z_i=1 for group = 1, Z_i=0 for group = 2.
\] \begin{align}
\frac{u(0)^2}{i(0)}&=\frac
{(\sum_{i=1}^{l}(S_i-\frac{\sum_{l\in R_{D_i}(\tau_i)}S_l}{\sum_{l\in R_{D_i}(\tau_i)}1}))^2}
{\sum_{i=1}^l\frac{(\sum_{l\in R_{D_i}(\tau_i)}S_l^2)(\sum_{l\in R_{D_i}(\tau_i)}1)-(\sum_{l\in R_{D_i}(\tau_i)}S_l)^2}{\{\sum_{l\in R_{D_i}(\tau_i)}1\}^2}}\\
&=\frac
{(\sum_{i=1}^{l}(d_{1i}-E(d_{1i})))^2}
{\sum_{i=1}^lE({d_{1i}}^2)-{E(d_{1i})}^2}\\
&=\frac
{(\sum_{i=1}^{l}(d_{1i}-\frac{n_{1i}d_i}{n_{1i}+n_{2i}}))^2}
{\sum_{i=1}^lvar(d_{1i})}\\
&=\frac
{(\sum_{i=1}^{l}(d_{1i}-\frac{n_{1i}d_i}{n_{1i}+n_{2i}}))^2}
{\sum_{i=1}^l\frac{d_in_{1i}n_{2i}(n_i-d_i)}{(n_i-1){n_i}^2}}\\
\end{align} \$\$

\end{document}
